src/derive.lean
@@ -1,5 +1,7 @@
 
+import tactic.monotonicity
 import serial
+import data.nat.serial
 import tactic.serial
 import tactic.norm_num
 import tactic.basic
@@ -8,6 +10,8 @@ import category.basic
 section tactic
 
 open tactic
+open tactic.interactive (unfold norm_num trivial simp ac_mono)
+open interactive
 
 meta def mk_up (u : level) (e : expr) : tactic expr :=
 do t  ← infer_type e,
@@ -33,59 +37,83 @@ do u' ← mk_meta_univ,
    let ulift_t : expr := expr.const ``ulift [u,u'],
    pure $ ulift_t t
 
-meta def mk_encode (u : level) : tactic (list (name × list (expr × expr))) :=
+meta def induction_state := (list (name × list ((expr × option expr) × expr)))
+
+meta def mk_encode (n : name) (u : level) : tactic $ bool × induction_state :=
 do x ← intro1,
-   vs ← cases_core x,
+   b ← is_recursive_type n,
+   when b $ do {
+     size ← to_expr ``(sizeof %%x) >>= mk_up u,
+     refine ``(encode %%size >> _) },
+   vs ← better_induction x,
    gs ← get_goals,
-   mzip_with (λ (g : ℕ × expr) (c : name × list expr × list (name × expr)),
+   prod.mk b <$> mzip_with (λ (g : ℕ × expr) (c : name × list (expr × option expr) × list (name × expr)),
      do let ⟨i,g⟩ := g,
         set_goals [g],
         when (gs.length ≠ 1) $ refine ``(write_word (fin.of_nat %%(reflect i)) >> _),
         let ⟨c,vs,_⟩ := c,
-        vs' ← vs.mmap infer_type,
+        vs' ← vs.mmap $ infer_type ∘ prod.fst,
         vs.mmap' (λ v,
-          do v ← mk_up u v,
-             refine ``(encode %%v >> _)),
+          do t ← infer_type v.1,
+             match v.2 with
+             | none := do
+               v ← mk_up u v.1,
+               refine ``(encode %%v >> _)
+             | (some rec_call) := do
+               refine ``(%%rec_call >> _)
+             end ),
         refine ``(pure punit.star),
         (c,vs.zip vs') <$ done) gs.enum vs
 
-meta def mk_parser (u : level) : expr → list (expr × expr) → list (name × expr) → tactic unit
-| e [] _ := refine ``(pure %%e)
-| e ((v,t) :: vs) σ :=
+meta def mk_parser (u : level) :
+  expr →
+  list ((expr × option expr) × expr) →
+  list (name × expr) →
+  option expr →
+  tactic unit
+| e [] _ rec_call := refine ``(pure %%e)
+| e (((v,rec),t) :: vs) σ rec_call :=
 do let t := t.instantiate_locals σ,
    ulift_t ← mk_ulift u t,
-   refine ``(decode %%ulift_t >>= _),
-   v' ← intro1,
-   v' ← mk_down u v' t,
-   mk_parser (e v') vs ( (v.local_uniq_name,v') :: σ )
+   v' ← match rec_call <* rec with
+   | none :=
+     do refine ``(decode %%ulift_t >>= _),
+        v' ← intro1,
+        mk_down u v' t
+   | (some rec_call) :=
+     refine ``(%%rec_call >>= _) >> intro1
+   end,
+   mk_parser (e v') vs ( (v.local_uniq_name,v') :: σ ) rec_call
 
-meta def mk_decode (u : level) (n : name) (pat : list (name × list (expr × expr))) : tactic unit :=
-do t ← target,
-   e ← get_env,
-   if pat.length = 1 then do
+meta def mk_decode (is_rec : bool) (args : list expr) (u : level) (n : name) (pat : induction_state) : tactic unit :=
+do if pat.length = 1 then do
        let ⟨c,vs⟩ := pat.head,
        c ← mk_const c,
-       mk_parser u c vs []
+       mk_parser u (c.mk_app args) vs [] none
    else do
+     rec_call ← if is_rec then do
+       nat_t ← mk_ulift u `(nat),
+       refine ``(decode %%nat_t >>= _),
+       n ← intro1,
+       refine ``(recursive_parser (ulift.down %%n) _),
+       some <$> intro `rec_call
+     else pure none,
      refine ``(select_tag _),
      pat.enum.mmap' $ λ ⟨i,c,vs⟩, do {
        v₀ ← mk_mvar, v₁ ← mk_mvar,
        refine ``((fin.of_nat %%(reflect i),%%v₀) :: %%v₁),
        set_goals [v₀],
        c ← mk_const c,
-       mk_parser u c vs [], done,
+       mk_parser u (c.mk_app args) vs [] rec_call, done,
        set_goals [v₁] },
      refine ``([])
-
--- set_option trace.app_builder true
-open tactic.interactive (unfold norm_num trivial)
-open interactive
 
 meta def reduce_select_tag (tag : expr) : expr → tactic unit
 | `( list.cons (fin.of_nat %%n, %%br) %%brs ) :=
   if n =ₐ tag then do
     v ← mk_mvar,
-    to_expr ``(read_write_tag_hit %%v) >>= rewrite_target,
+    to_expr ``(read_write_tag_hit %%v) >>= rewrite_target <|>
+      (to_expr ``(read_write_tag_hit' %%v) >>= rewrite_target),
     gs ← get_goals,
     set_goals [v], tactic.interactive.norm_num [] (loc.ns [none]), done,
     set_goals gs
@@ -105,22 +133,76 @@ meta def reduce_select_tag (tag : expr) : expr → tactic unit
 meta def match_sum_branch : tactic unit :=
 do brs ← mk_mvar, tag ← mk_mvar,
    tgt ← target,
-   to_expr ``(select_tag %%brs -<< (write_word (fin.of_nat %%tag) >>= _) = _) >>= unify tgt,
-   brs ← instantiate_mvars brs,
-   tag ← instantiate_mvars tag,
-   reduce_select_tag tag brs
+   mcond (succeeds $
+     to_expr ``(select_tag %%brs -<< (write_word (fin.of_nat %%tag) >> _) = _) >>= change <|>
+       (to_expr ``(select_tag %%brs -<< (write_word (fin.of_nat %%tag)) = _) >>= change))
+   (do brs ← instantiate_mvars brs,
+       tag ← instantiate_mvars tag,
+       reduce_select_tag tag brs)
+   skip
 
-meta def mk_serial_correctness (encode_n decode_n : name) : tactic unit :=
-do w ← intro1, cases w,
-   all_goals $ do {
-     dunfold_target [decode_n,encode_n],
-     match_sum_branch <|> skip,
-     `[simp [(>>),encode_decode_bind,encode_decode_bind',encode_decode_pure]],
-     done }
+meta def prove_bound (n : name) : tactic unit :=
+solve1 $ do
+  h ← get_local `h,
+  transitivity; [skip, () <$ apply h],
+  dunfold_target [``sizeof],
+  dunfold_target [``sizeof,``has_sizeof.sizeof,n <.> "sizeof"],
+  try $ to_expr  ``(1 + 0 ≤ _) >>= change,
+  (`[ac_mono*]; try ( applyc ``nat.zero_le) ) <|> reflexivity,
+  done <|> do {
+    repeat $ applyc ``nat.le_add_right <|> applyc ``nat.le_add_of_le_left,
+    try $ reflexivity },
+  return ()
+
+meta def mk_serial_correctness (is_rec : bool) (n encode_n decode_n : name) : tactic unit :=
+do let rules := [``has_bind.and_then,
+                 ``encode_decode_bind,``encode_decode_bind',
+                 ``encode_decode_pure],
+   rules ← rules.mmap ((<$>) simp_arg_type.expr ∘ resolve_name),
+   w ← intro1,
+   dunfold_target [decode_n],
+   dunfold_target [encode_n],
+   simp none ff rules [] (loc.ns [none]),
+   hs ← if is_rec then
+   do { tactic.interactive.generalize `h () (``(sizeof %%w),`k),
+        k ← get_local `k,
+        h ← get_local `h,
+        replace `h ``(le_of_eq %%h),
+        revert k,
+        better_induction w <* all_goals (() <$ intro_lst [`k,`h]) }
+   else better_induction w,
+   gs ← get_goals,
+   mzip_with' (λ g (h : name × list (expr × option expr) × list (name × expr)), do {
+     set_goals [g],
+     let ⟨_,ih,_⟩ := h,
+     let ih := ih.filter_map prod.snd,
+     when is_rec $ `[rw recursive_parser_unfold],
+     solve1 $ do {
+       match_sum_branch,
+       ih.mmap' $ λ hh,
+       do { try $ simp none ff rules [] (loc.ns [none]),
+            bound ← mk_mvar,
+            mcond (succeeds $ to_expr ``((_ >>= _) -<< (_ >> _) = _) >>= change)
+              (do dunfold_target [``has_bind.and_then],
+                  to_expr ``(read_write_mono $ %%hh _ %%bound) >>= rewrite_target)
+              (do to_expr ``((_ >>= _) -<< _ = _) >>= change,
+                  to_expr ``(read_write_mono_left $ %%hh _ %%bound) >>= rewrite_target),
+            gs ← get_goals, set_goals [bound],
+            h ← get_local `h,
+            applyc ``nat.le_sub_right_of_add_le,
+            prove_bound n,
+            set_goals gs },
+       simp none ff rules [] (loc.ns [none]) <|> reflexivity },
+     when is_rec $ prove_bound n,
+     done,
+     pure ()
+   }) gs hs
 
 meta def mk_serial_instance : tactic unit :=
+expand_untrusted $
 do tgt ← target,
    let t := tgt.app_arg,
+   let args := t.get_app_args,
    (expr.sort (level.succ u)) ← infer_type t,
    let n := t.get_app_fn.const_name,
    d ← get_decl n,
@@ -128,19 +210,20 @@ do tgt ← target,
    enc ← mk_mvar,
    dec ← mk_mvar,
    correct ← mk_mvar,
+   reset_instance_cache,
    refine ``( { encode := %%enc,
                 decode := %%dec,
                 correctness := %%correct } ),
    let decode_n := n <.> "decode",
    let encode_n := n <.> "encode",
    set_goals [enc],
-   vs ← extract_def' encode_n t (mk_encode u),
+   (is_rec,vs) ← extract_def' encode_n t (mk_encode n u),
    set_goals [dec],
-   extract_def' decode_n t (mk_decode u n vs),
+   extract_def' decode_n t (mk_decode is_rec args u n vs),
    set_goals [correct],
-   mk_serial_correctness encode_n decode_n
+   mk_serial_correctness is_rec n encode_n decode_n
 
-@[derive_handler] meta def serial_derive_handler :=
+@[derive_handler] meta def serial_derive_handler : derive_handler :=
 instance_derive_handler ``serial mk_serial_instance
 
 end tactic
@@ -156,3 +239,8 @@ structure my_struct :=
 (x : ℕ)
 (xs : list ℕ)
 (bounded : xs.length ≤ x)
+
+@[derive serial]
+inductive tree (α : Type)
+| leaf : tree
+| node2 : α → tree → tree → tree
