src/medium.lean
@@ -263,9 +263,9 @@ begin
     rw [x₁_ih _ _ _ h], }
 end
 
-lemma read_write_mono {α β} (i : α)
-      (x₀ : get_m α) (f₀ : α → get_m β)
-      (x₁ : put_m) (f₁ : punit → put_m)
+lemma read_write_mono {α β} {i : α}
+      {x₀ : get_m α} {f₀ : α → get_m β}
+      {x₁ : put_m} {f₁ : punit → put_m}
       (h : x₀ -<< x₁ = some i) :
   (x₀ >>= f₀) -<< (x₁ >>= f₁) = f₀ i -<< f₁ punit.star :=
 begin
@@ -276,12 +276,12 @@ begin
   simp [h],
 end
 
-lemma read_write_mono_left {α β} (i : α)
-      (x₀ : get_m α) (f₀ : α → get_m β)
-      (x₁ : put_m)
+lemma read_write_mono_left {α β} {i : α}
+      {x₀ : get_m α} {f₀ : α → get_m β}
+      {x₁ : put_m}
       (h : x₀ -<< x₁ = some i) :
   (x₀ >>= f₀) -<< x₁ = f₀ i -<< pure punit.star :=
-by rw ← read_write_mono _ x₀ f₀ x₁ pure h; simp
+by rw ← read_write_mono h; simp
 
 lemma read_write_eq_eval_eval {α}
       (x₀ : get_m α) (x₁ : put_m)  :
